thys-2019/sepref/IICF/IICF.thy
@@ -32,5 +32,55 @@ imports
 
 
 begin
-  thy_deps
+
+subsection \<open>Regression Tests\<close>  
+experiment
+begin
+  (* TODO: Augment! *)
+
+  text \<open>Free parameter\<close>
+  sepref_definition test_free1 is "\<lambda>xs. doN { 
+    ASSERT(length xs = 10); 
+    r \<leftarrow> mop_list_get xs 1;
+    mop_free xs;
+    RETURN r
+  }" :: "(array_assn bool1_assn)\<^sup>d \<rightarrow>\<^sub>a bool1_assn"
+    apply (annot_snat_const "TYPE(64)")
+    by sepref
+
+  
+  text \<open>Free bound var before it goes out of scope\<close>
+  sepref_definition test_free2 is "\<lambda>N. doN { 
+    ASSERT(N>10); 
+    xs \<leftarrow> mop_array_custom_replicate N False;
+    xs \<leftarrow> mop_list_set xs 3 True;
+    r1 \<leftarrow> mop_list_get xs 2;
+    r2 \<leftarrow> mop_list_get xs 3;
+    mop_free xs;
+    xs \<leftarrow> mop_array_custom_replicate N False;
+    RETURN (r1 \<and> r2) 
+  }" :: "(snat_assn' TYPE(64))\<^sup>k \<rightarrow>\<^sub>a bool1_assn"
+    apply (annot_snat_const "TYPE(64)")
+    by sepref
+    
+  text \<open>Free bound var + parameter\<close>
+  sepref_definition test_free3 is "\<lambda>xs. doN { 
+    ASSERT(length xs = 10); 
+    xs2 \<leftarrow> mop_array_custom_replicate 10 False;
+    xs2 \<leftarrow> mop_list_set xs2 3 True;
+    r1 \<leftarrow> mop_list_get xs2 1;
+    mop_free xs2;
+    r2 \<leftarrow> mop_list_get xs 1;
+    mop_free xs;
+    RETURN (r1 \<and> r2) 
+  }" :: "(array_assn bool1_assn)\<^sup>d \<rightarrow>\<^sub>a bool1_assn"
+    apply (annot_snat_const "TYPE(64)")
+    by sepref
+  
+
+
+end
+
+
+
 end
